Fix some errors in cohen_poset.lean
Fix some more errors

Fix errors

src/cohen_poset.lean
@@ -1,12 +1,12 @@
-import .fol data.pfun data.set tactic.tidy data.set.countable data.set.basic .to_mathlib        
+import data.pfun data.set tactic.tidy data.set.countable data.set.basic .to_mathlib pSet_ordinal
 -- local attribute [instance] classical.prop_decidable
-open fol
 
 /- The Cohen poset of finite partial functions (2^(2^ω)) × ω → 2 -/
 
 /- The underlying type of the Cohen poset is the type of finite partial functions from (set $ set ω) × ω → Prop -/
+variable {η : cardinal}
 
-def cohen_poset := {f : ((set $ set ℕ) × ℕ) →. Prop | set.finite (pfun.dom f)}
+def cohen_poset := {f : ((pSet.ordinal.mk η.ord).type × ℕ) →. Prop | set.finite (pfun.dom f)}
 
 -- TODO replace all instances of set $ set ℕ with a generic "B"
 noncomputable instance B_decidable_eq : decidable_eq (set $ set ℕ) := λ _ _, classical.prop_decidable _
@@ -87,7 +87,7 @@ lemma lift_graph' {α β : Type*} {f : α →. β} {a : α} {b : β} (h_a : a �
 end pfun
 
 /- Partial order structure on the Cohen poset -/
-instance partial_order_cohen_poset : partial_order cohen_poset :=
+instance partial_order_cohen_poset : partial_order (@cohen_poset η) :=
 { le := λ f g, g.val.graph ⊆ f.val.graph,
   lt := λ f g, g.val.graph ⊆ f.val.graph ∧ ¬ f.val.graph ⊆ g.val.graph,
   le_refl := λ _, by unfold has_le.le,
@@ -179,17 +179,17 @@ end
 noncomputable instance Prop_encodable : encodable Prop :=
  @encodable.of_equiv _ _ (by apply_instance) equiv_Prop_bool
 
-noncomputable def size_of_domain : cohen_poset → ℕ :=
+noncomputable def size_of_domain : (@cohen_poset η) → ℕ :=
   λ p, finset.card $ set.finite.to_finset p.property
 
-lemma size_of_domain_fiber {n} {p : cohen_poset} (h : p ∈ size_of_domain ⁻¹' {n}) : size_of_domain p = n := by finish
+lemma size_of_domain_fiber {n} {p : @cohen_poset η} (h : p ∈ @size_of_domain η ⁻¹' {n}) : size_of_domain p = n := by finish
 
 /-- The partial function p is defined at b and m if (b,m) is in the domain of p -/
-def is_defined (p : cohen_poset) (b) (m) := (b,m) ∈ (pfun.dom p.val)
+def is_defined (p : (@cohen_poset η)) (b) (m) := (b,m) ∈ (pfun.dom p.val)
 
 /-- p is defined at m if there exists a b such that p is defined at b and m -/
-def is_defined_at (m : ℕ) : set cohen_poset :=
-  {p : cohen_poset | ∃ b, is_defined p b m}
+def is_defined_at (m : ℕ) : set (@cohen_poset η) :=
+  {p : (@cohen_poset η) | ∃ b, is_defined p b m}
 
 namespace finset
 
@@ -201,13 +201,13 @@ end
 
 end finset
 
-lemma empty_of_size_of_domain_0 {p : cohen_poset} (h : size_of_domain p = 0) : p.val.dom = ∅ :=
+lemma empty_of_size_of_domain_0 {p : (@cohen_poset η)} (h : size_of_domain p = 0) : p.val.dom = ∅ :=
 begin
   have : set.finite.to_finset p.property = ∅, from finset.card_eq_zero.mp h,
   exact finset.empty_of_empty this
 end
 
-lemma nonempty_of_size_of_domain_ne_zero {p : cohen_poset} (h : size_of_domain p ≠ 0) : nonempty p.val.dom :=
+lemma nonempty_of_size_of_domain_ne_zero {p : (@cohen_poset η)} (h : size_of_domain p ≠ 0) : nonempty p.val.dom :=
 begin
   have : set.finite.to_finset p.property ≠ ∅, by {intro h, suffices : (set.finite.to_finset p.property).card = 0,
     by {apply (_root_.not_and_self ((set.finite.to_finset p.property).card = 0)).mp,refine ⟨(by assumption), this⟩},
@@ -216,7 +216,7 @@ begin
   refine ⟨this_w,_⟩, cases this_w, cases p, simp at this_h, assumption
 end
 
-lemma nonempty_domain_defined (p : cohen_poset) (h : 0 < size_of_domain p) : ∃ m,
+lemma nonempty_domain_defined (p : (@cohen_poset η)) (h : 0 < size_of_domain p) : ∃ m,
   is_defined_at m p :=
 begin
   suffices : nonempty p.val.dom, by {have := classical.choice this, cases this,
@@ -224,20 +224,20 @@ begin
   intro h', rw[h'] at h, cases h
 end
 
-def is_defined_at_covers {n} {h : 0 < n} : size_of_domain ⁻¹' {n} ⊆ ⋃ m, is_defined_at m :=
-begin
-  intros p Hp, simp[set.mem_preimage_eq] at *,
-  suffices : nonempty p.val.dom,
-    by {have := classical.choice this, exact ⟨this.val.snd, ⟨this.val.fst, (by tidy)⟩⟩},
-  apply nonempty_of_size_of_domain_ne_zero, intro H, have : 0 < 0, by cc, cases this
-end
+-- def is_defined_at_covers {n} {h : 0 < n} : @size_of_domain η ⁻¹' {n} ⊆ ⋃ m, is_defined_at m :=
+-- begin
+--   intros p Hp, simp[set.mem_preimage_eq] at *,
+--   suffices : nonempty p.val.dom,
+--     by {have := classical.choice this, exact ⟨this.val.snd, ⟨this.val.fst, (by tidy)⟩⟩},
+--   apply nonempty_of_size_of_domain_ne_zero, intro H, have : 0 < 0, by cc, cases this
+-- end
 
-instance size_of_domain_0_subsingleton : subsingleton $ size_of_domain ⁻¹' {0} :=
+instance size_of_domain_0_subsingleton : subsingleton $ @size_of_domain η ⁻¹' {0} :=
 begin
   refine ⟨λ a b, _⟩, rcases a with ⟨⟨p_a, H_f_a⟩, H_a⟩, rcases b with ⟨⟨p_b, H_f_b⟩, H_b⟩, congr,
-  have := (pfun.graph_empty_iff_dom_empty _).mpr (@empty_of_size_of_domain_0 _
+  have := (pfun.graph_empty_iff_dom_empty _).mpr (@empty_of_size_of_domain_0 η _
                                           (by {simp[set.mem_preimage_eq] at H_b, exact H_b})),
-  have := (pfun.graph_empty_iff_dom_empty _).mpr (@empty_of_size_of_domain_0 _
+  have := (pfun.graph_empty_iff_dom_empty _).mpr (@empty_of_size_of_domain_0 η _
                                           (by {simp[set.mem_preimage_eq] at H_a, exact H_a})),
   exact pfun.ext_graph _ _ (by cc)
 end
@@ -249,16 +249,16 @@ begin
   suffices : f a = f b, by tidy, apply this, exact x.property
 end
 
-lemma size_of_domain_0_inter_subsingleton : ∀ (a : set cohen_poset), subsingleton ↥((size_of_domain ⁻¹' {0}) ∩ a) :=
+lemma size_of_domain_0_inter_subsingleton : ∀ (a : set (@cohen_poset η)), subsingleton ↥((size_of_domain ⁻¹' {0}) ∩ a) :=
 λ a, subsingleton_of_subset_of_subsingleton
      (by apply set.inter_subset_left : size_of_domain ⁻¹' {0} ∩ a ⊆ size_of_domain ⁻¹' {0})
 
 lemma countable_subsingleton {α : Type*} (s : set α) (h : subsingleton s) : set.countable s :=
   set.countable_iff_exists_injective.mpr $ ⟨λ _, 0, λ _ _, dec_trivial⟩
 
-lemma cover_Union_eq {α ι : Type*} {s : set α} {t : ι → set α} {h : s ⊆ ⋃ i, t i} :
-s = ⋃ i, s ∩ t i :=
-  by {rw[<-set.inter_Union_left], ext, split; intros, exact ⟨a, h a⟩, exact a.left}
+-- lemma cover_Union_eq {α ι : Type*} {s : set α} {t : ι → set α} {h : s ⊆ (⋃ (i : ι), t i)} :
+-- s = ⋃ i, s ∩ t i :=
+--   by {rw[<-set.inter_Union_left], ext, split; intros, exact ⟨a, h a⟩, exact a.left}
 
 lemma inter_subset_left' {α : Type*} {s t u : set α} {h : t ⊆ u} : s ∩ t ⊆ u :=
   λ _ ⟨_,_⟩, by solve_by_elim
@@ -282,278 +282,279 @@ def pfun.restriction {α β : Type*} (f : α →. β) (s : set α) : α →. β
 lemma pfun.domain_restriction {α β : Type*} {f : α →. β} {s : set α} : (pfun.restriction f s).dom = f.dom ∩ s :=
   by ext; split; intro a; cases a; fsplit; assumption
 
-def one_point_restriction (p : cohen_poset) : ∀(x), x ∈ p.val.dom → cohen_poset :=
-λ x H, ⟨pfun.restriction p.val (not_x x),
-         by {change set.finite (pfun.restriction p.val (not_x x)).dom,
-         rw[pfun.domain_restriction], apply finite_of_inter_not_x, apply p.property}⟩
+end one_point_restriction
+-- def one_point_restriction (p : (@cohen_poset η)) : ∀(x), x ∈ p.val.dom → (@cohen_poset η) :=
+-- λ x H, ⟨pfun.restriction p.val (not_x x),
+--          by {change set.finite (pfun.restriction p.val (not_x x)).dom,
+--          rw[pfun.domain_restriction], apply finite_of_inter_not_x, apply p.property}⟩
 
-def one_point_restriction' (p : cohen_poset) : ∀ (x), cohen_poset :=
-λ x, ⟨pfun.restriction p.val (not_x x),
-         by {change set.finite (pfun.restriction p.val (not_x x)).dom,
-         rw[pfun.domain_restriction], apply finite_of_inter_not_x, apply p.property}⟩
+-- def one_point_restriction' (p : (@cohen_poset η)) : ∀ (x), (@cohen_poset η) :=
+-- λ x, ⟨pfun.restriction p.val (not_x x),
+--          by {change set.finite (pfun.restriction p.val (not_x x)).dom,
+--          rw[pfun.domain_restriction], apply finite_of_inter_not_x, apply p.property}⟩
 
-lemma one_point_restriction_domain {p : cohen_poset} {x} (h : x ∈ p.val.dom) : (one_point_restriction p x h).val.dom = p.val.dom ∩ not_x x :=
-begin
-  ext, split; {intros a, auto_cases, fsplit; assumption}
-end
-
-lemma one_point_restriction_domain' {p : cohen_poset} {x} : (one_point_restriction' p x).val.dom = p.val.dom ∩ not_x x :=
-begin
-  ext, split; {intros a, auto_cases, fsplit; assumption}
-end
-
-lemma one_point_restriction_graph {p : cohen_poset} {x} {h_x : x ∈ p.val.dom} : ∀ y, y ∈ (one_point_restriction p x h_x).val.graph ↔ (y ∈ p.val.graph ∧ (prod.fst y ≠ x)) := sorry
-
--- lemma one_point_restriction_graph' {p : cohen_poset} {x} : (one_point_restriction' p x).val.graph = {y ∈ p.val.graph | y.fst ∈ not_x x} :=
+-- lemma one_point_restriction_domain {p : (@cohen_poset η)} {x} (h : x ∈ p.val.dom) : (one_point_restriction p x h).val.dom = p.val.dom ∩ not_x x :=
 -- begin
---   ext, split; intros, 
+--   ext, split; {intros a, auto_cases, fsplit; assumption}
 -- end
 
-@[simp]lemma in_one_point_restriction_of_in_dom_and_not_x {p : cohen_poset} {x} {h : x ∈ p.val.dom} {y} : y ∈ (one_point_restriction p x h).val.dom ↔ (y ∈ p.val.dom) ∧ y ≠ x :=
-  by simp[one_point_restriction_domain, not_x]; finish
+-- lemma one_point_restriction_domain' {p : (@cohen_poset η)} {x} : (one_point_restriction' p x).val.dom = p.val.dom ∩ not_x x :=
+-- begin
+--   ext, split; {intros a, auto_cases, fsplit; assumption}
+-- end
 
-@[simp]lemma in_one_point_restriction'_of_in_dom_and_not_x {p : cohen_poset} {x} {y} : y ∈ (one_point_restriction' p x ).val.dom ↔ (y ∈ p.val.dom) ∧ y ≠ x :=
-  by simp[one_point_restriction_domain', not_x]; finish
+-- lemma one_point_restriction_graph {p : (@cohen_poset η)} {x} {h_x : x ∈ p.val.dom} : ∀ y, y ∈ (one_point_restriction p x h_x).val.graph ↔ (y ∈ p.val.graph ∧ (prod.fst y ≠ x)) := sorry
 
-lemma one_point_restriction_domain'_subset {p : cohen_poset} {x} : (one_point_restriction' p x).val.dom ⊆ p.val.dom :=
-  λ y, by finish
+-- -- lemma one_point_restriction_graph' {p : (@cohen_poset η)} {x} : (one_point_restriction' p x).val.graph = {y ∈ p.val.graph | y.fst ∈ not_x x} :=
+-- -- begin
+-- --   ext, split; intros, 
+-- -- end
 
-lemma one_point_restriction_domain_subset {p : cohen_poset} {x} {h_x : x ∈ p.val.dom} : (one_point_restriction p x h_x).val.dom ⊆ p.val.dom :=
-  λ y, by finish
+-- @[simp]lemma in_one_point_restriction_of_in_dom_and_not_x {p : (@cohen_poset η)} {x} {h : x ∈ p.val.dom} {y} : y ∈ (one_point_restriction p x h).val.dom ↔ (y ∈ p.val.dom) ∧ y ≠ x :=
+--   by simp[one_point_restriction_domain, not_x]; finish
+
+-- @[simp]lemma in_one_point_restriction'_of_in_dom_and_not_x {p : (@cohen_poset η)} {x} {y} : y ∈ (one_point_restriction' p x ).val.dom ↔ (y ∈ p.val.dom) ∧ y ≠ x :=
+--   by simp[one_point_restriction_domain', not_x]; finish
+
+-- lemma one_point_restriction_domain'_subset {p : (@cohen_poset η)} {x} : (one_point_restriction' p x).val.dom ⊆ p.val.dom :=
+--   λ y, by finish
+
+-- lemma one_point_restriction_domain_subset {p : (@cohen_poset η)} {x} {h_x : x ∈ p.val.dom} : (one_point_restriction p x h_x).val.dom ⊆ p.val.dom :=
+--   λ y, by finish
 
 
-lemma one_point_restriction_domain_coe {p : cohen_poset} {x} {h : x ∈ p.val.dom} : p.val.dom = ↑(set.finite.to_finset p.property) := by simp
+-- lemma one_point_restriction_domain_coe {p : (@cohen_poset η)} {x} {h : x ∈ p.val.dom} : p.val.dom = ↑(set.finite.to_finset p.property) := by simp
 
-lemma one_point_restriction_finset_rewrite {p : cohen_poset} {x} {h : x ∈ p.val.dom} : set.finite.to_finset (one_point_restriction p x h).property = set.finite.to_finset (by {apply finite_of_inter_not_x, exact p.property} : set.finite $ p.val.dom ∩ not_x x) := by simp[one_point_restriction_domain]
+-- lemma one_point_restriction_finset_rewrite {p : (@cohen_poset η)} {x} {h : x ∈ p.val.dom} : set.finite.to_finset (one_point_restriction p x h).property = set.finite.to_finset (by {apply finite_of_inter_not_x, exact p.property} : set.finite $ p.val.dom ∩ not_x x) := by simp[one_point_restriction_domain]
 
-lemma one_point_restriction_finset_rewrite_property {p : cohen_poset} {x} {h : x ∈ p.val.dom} : ∀ y, y ∈ set.finite.to_finset ((one_point_restriction p x h).property-- by {apply finite_of_inter_not_x, exact p.property} : set.finite $ p.val.dom ∩ not_x x
-) ↔ y ≠ x ∧ y ∈ p.val.dom :=
-begin
-  intro y, split; intros, rw[one_point_restriction_finset_rewrite] at a, split,
-    {tidy, apply a_right, refl},
-    {finish},
-    {apply finset.mem_coe.mp, rw[<-one_point_restriction_domain_coe],
-    rw[one_point_restriction_domain], refine ⟨a.right,_⟩, apply a.left, swap, exact y, simp*}
-end
+-- lemma one_point_restriction_finset_rewrite_property {p : (@cohen_poset η)} {x} {h : x ∈ p.val.dom} : ∀ y, y ∈ set.finite.to_finset ((one_point_restriction p x h).property-- by {apply finite_of_inter_not_x, exact p.property} : set.finite $ p.val.dom ∩ not_x x
+-- ) ↔ y ≠ x ∧ y ∈ p.val.dom :=
+-- begin
+--   intro y, split; intros, rw[one_point_restriction_finset_rewrite] at a, split,
+--     {tidy, apply a_right, refl},
+--     {finish},
+--     {apply finset.mem_coe.mp, rw[<-one_point_restriction_domain_coe],
+--     rw[one_point_restriction_domain], refine ⟨a.right,_⟩, apply a.left, swap, exact y, simp*}
+-- end
 
-lemma one_point_restriction_erase {p : cohen_poset} {x} {h : x ∈ p.val.dom} : set.finite.to_finset (one_point_restriction p x h).property = finset.erase (set.finite.to_finset p.property) x :=
-begin
-  ext, rw[one_point_restriction_finset_rewrite,finset.mem_erase], conv {to_rhs,rw[<-finset.mem_coe]}, split; intros, {rw[<-one_point_restriction_domain_coe], apply (one_point_restriction_finset_rewrite_property a).mp, show set (set ℕ) × ℕ, exact x, rw[one_point_restriction_finset_rewrite], repeat{assumption}},
-  {rw[<-one_point_restriction_finset_rewrite],
-  apply (one_point_restriction_finset_rewrite_property a).mpr,
-  convert a_1, simp, assumption}
-end
+-- lemma one_point_restriction_erase {p : (@cohen_poset η)} {x} {h : x ∈ p.val.dom} : set.finite.to_finset (one_point_restriction p x h).property = finset.erase (set.finite.to_finset p.property) x :=
+-- begin
+--   ext, rw[one_point_restriction_finset_rewrite,finset.mem_erase], conv {to_rhs,rw[<-finset.mem_coe]}, split; intros, {rw[<-one_point_restriction_domain_coe], apply (one_point_restriction_finset_rewrite_property a).mp, show set (set ℕ) × ℕ, exact x, rw[one_point_restriction_finset_rewrite], repeat{assumption}},
+--   {rw[<-one_point_restriction_finset_rewrite],
+--   apply (one_point_restriction_finset_rewrite_property a).mpr,
+--   convert a_1, simp, assumption}
+-- end
 
-lemma one_point_restriction_decrease_size {n} (p : cohen_poset) (h : size_of_domain p = n + 1) (x) (h_x : x ∈ p.val.dom)  :
-size_of_domain (one_point_restriction p x h_x) = n :=
-begin
-  unfold size_of_domain at *, have : n = nat.pred (n+1), by refl,
-  rw[this, one_point_restriction_erase, <-h], apply finset.card_erase_of_mem,
-  apply finset.mem_coe.mp, rwa[finset.coe_to_finset]
-end
+-- lemma one_point_restriction_decrease_size {n} (p : (@cohen_poset η)) (h : size_of_domain p = n + 1) (x) (h_x : x ∈ p.val.dom)  :
+-- size_of_domain (one_point_restriction p x h_x) = n :=
+-- begin
+--   unfold size_of_domain at *, have : n = nat.pred (n+1), by refl,
+--   rw[this, one_point_restriction_erase, <-h], apply finset.card_erase_of_mem,
+--   apply finset.mem_coe.mp, rwa[finset.coe_to_finset]
+-- end
 
-def aux_c'' {p₁ p₂ : cohen_poset} {t₁ t₂ : (set $ set ℕ) × ℕ} (h_t₁ : t₁ ∈ p₁.val.dom) (h_t₂ : t₂ ∈ p₂.val.dom) (q : Prop) (h_val₁ : pfun.fn p₁.val t₁ h_t₁ = q) (h_val₂ : pfun.fn p₂.val t₂ h_t₂ = q) (c : cohen_poset) : cohen_poset :=
-  (one_point_restriction' (one_point_restriction' c t₁) t₂)
+-- def aux_c'' {p₁ p₂ : (@cohen_poset η)} {t₁ t₂ : (set $ set ℕ) × ℕ} (h_t₁ : t₁ ∈ p₁.val.dom) (h_t₂ : t₂ ∈ p₂.val.dom) (q : Prop) (h_val₁ : pfun.fn p₁.val t₁ h_t₁ = q) (h_val₂ : pfun.fn p₂.val t₂ h_t₂ = q) (c : (@cohen_poset η)) : (@cohen_poset η) :=
+--   (one_point_restriction' (one_point_restriction' c t₁) t₂)
 
-lemma aux_c''_dom {p₁ p₂ : cohen_poset} {t₁ t₂ : (set $ set ℕ) × ℕ} {h_t₁ : t₁ ∈ p₁.val.dom} {h_t₂ : t₂ ∈ p₂.val.dom} {q : Prop} {h_val₁ : pfun.fn p₁.val t₁ h_t₁ = q} {h_val₂ : pfun.fn p₂.val t₂ h_t₂ = q} {c : cohen_poset} : ∀ (x), x ∈ (aux_c'' h_t₁ h_t₂ q h_val₁ h_val₂ c).val.dom → x ≠ t₁ ∧ x ≠ t₂ :=
-λ x Hx, ⟨by {apply ((in_one_point_restriction'_of_in_dom_and_not_x).mp _).right, exact c,
-            apply one_point_restriction_domain'_subset, swap, exact t₂, exact Hx},
-         by {apply ((in_one_point_restriction'_of_in_dom_and_not_x).mp _).right, exact (one_point_restriction' c t₁), exact Hx}⟩  
-
-lemma aux_c''_dom_of {p₁ p₂ : cohen_poset} {t₁ t₂ : (set $ set ℕ) × ℕ} {h_t₁ : t₁ ∈ p₁.val.dom} {h_t₂ : t₂ ∈ p₂.val.dom} {q : Prop} {h_val₁ : pfun.fn p₁.val t₁ h_t₁ = q} {h_val₂ : pfun.fn p₂.val t₂ h_t₂ = q} {c : cohen_poset} : ∀ (x), x ≠ t₁ ∧ x ≠ t₂ → x ∈ c.val.dom → x ∈ (aux_c'' h_t₁ h_t₂ q h_val₁ h_val₂ c).val.dom :=
-begin
-  intros x Hx H'x, rcases Hx with ⟨Hx_r, Hx_l⟩, dsimp[aux_c''],
-  repeat{rw[one_point_restriction_domain']}, finish
-end
-
-lemma aux_c''_graph_of {p₁ p₂ : cohen_poset} {t₁ t₂ : (set $ set ℕ) × ℕ} {h_t₁ : t₁ ∈ p₁.val.dom} {h_t₂ : t₂ ∈ p₂.val.dom} {q : Prop} {h_val₁ : pfun.fn p₁.val t₁ h_t₁ = q} {h_val₂ : pfun.fn p₂.val t₂ h_t₂ = q} {c : cohen_poset} : ∀ x, (x ∈ c.val.graph ∧ (prod.fst x ≠ t₁ ) ∧ (prod.fst x ≠ t₂)) ↔ x ∈ (aux_c'' h_t₁ h_t₂ q h_val₁ h_val₂ c).val.graph := sorry
-
-lemma aux_c''_dom_finite {p₁ p₂ : cohen_poset} {t₁ t₂ : (set $ set ℕ) × ℕ} {h_t₁ : t₁ ∈ p₁.val.dom} {h_t₂ : t₂ ∈ p₂.val.dom} {q : Prop} {h_val₁ : pfun.fn p₁.val t₁ h_t₁ = q} {h_val₂ : pfun.fn p₂.val t₂ h_t₂ = q} {c : cohen_poset} : set.finite (aux_c'' h_t₁ h_t₂ q h_val₁ h_val₂ c).val.dom :=
-begin
-  dsimp[aux_c''], repeat{rw[one_point_restriction_domain']}, repeat{apply finite_of_inter_not_x},
-  exact c.property
-end
+-- lemma aux_c''_dom {p₁ p₂ : (@cohen_poset η)} {t₁ t₂ : (set $ set ℕ) × ℕ} {h_t₁ : t₁ ∈ p₁.val.dom} {h_t₂ : t₂ ∈ p₂.val.dom} {q : Prop} {h_val₁ : pfun.fn p₁.val t₁ h_t₁ = q} {h_val₂ : pfun.fn p₂.val t₂ h_t₂ = q} {c : (@cohen_poset η)} : ∀ (x), x ∈ (aux_c'' h_t₁ h_t₂ q h_val₁ h_val₂ c).val.dom → x ≠ t₁ ∧ x ≠ t₂ :=
 -- λ x Hx, ⟨by {apply ((in_one_point_restriction'_of_in_dom_and_not_x).mp _).right, exact c,
 --             apply one_point_restriction_domain'_subset, swap, exact t₂, exact Hx},
---          by {apply ((in_one_point_restriction'_of_in_dom_and_not_x).mp _).right, exact (one_point_restriction' c t₁), exact Hx}⟩
+--          by {apply ((in_one_point_restriction'_of_in_dom_and_not_x).mp _).right, exact (one_point_restriction' c t₁), exact Hx}⟩  
 
-/- Let p₁ and p₂ be two partial functions such that there is a point (b₁,m) for p₁ and a point (b₂, m) for p₂ where p₁ and p₂ have the same value.
-    Suppose that the one-point restrictions of p₁ and p₂ with respect to (b₁,m) and (b₂,m) have a common refinement c.
-    Then c (after making sure (b₁, m) and (b₂,m) are not in its domain) extended by (b₁,m) and (b₂,m) is a common refinement for p₁ and p₂. -/
-
-/-- the graph of the extension of c by (b₁,m) and (b₂,m) -/
-def one_point_restriction_refinement_extension_graph {p₁ p₂ : cohen_poset} {t₁ t₂ : (set $ set ℕ) × ℕ} (h_t₁ : t₁ ∈ p₁.val.dom) (h_t₂ : t₂ ∈ p₂.val.dom) (q : Prop) (h_val₁ : pfun.fn p₁.val t₁ h_t₁ = q) (h_val₂ : pfun.fn p₂.val t₂ h_t₂ = q) (c : cohen_poset) :=
-  ((aux_c'' h_t₁ h_t₂ q h_val₁ h_val₂ c).val.graph ∪ {(t₁,q)} ∪ {(t₂,q)})
-
-lemma one_point_restriction_refinement_extension_graph_functional {p₁ p₂ : cohen_poset} {t₁ t₂ : (set $ set ℕ) × ℕ} (h_t₁ : t₁ ∈ p₁.val.dom) (h_t₂ : t₂ ∈ p₂.val.dom) (q : Prop) (h_val₁ : pfun.fn p₁.val t₁ h_t₁ = q) (h_val₂ : pfun.fn p₂.val t₂ h_t₂ = q) (c : cohen_poset) (h_c_left : c ≤ (one_point_restriction p₁ t₁ h_t₁)) (h_c_right : c ≤ (one_point_restriction p₂ t₂ h_t₂)) :
-  pfun.functional $ one_point_restriction_refinement_extension_graph h_t₁ h_t₂ q h_val₁ h_val₂ c :=
-begin
-  intros x q₁ q₂ H₁ H₂, let c' := (aux_c'' h_t₁ h_t₂ q h_val₁ h_val₂ c), cases H₁; cases H₂; cases H₁; cases H₂,
-  apply pfun.graph_functional (aux_c'' h_t₁ h_t₂ q h_val₁ h_val₂ c).val, exact H₁, exact H₂,
-  {have : x ∈ c'.val.dom,
-    by {apply (pfun.dom_iff_graph c'.val x).mpr, exact ⟨q₁, H₁⟩}, have := (aux_c''_dom x this).left, suffices : x = t₁, by contradiction, repeat{cases H₂}, refl},
-  {repeat{cases H₁}, suffices : t₁ ≠ t₁, by contradiction, have : t₁ ∈ c'.val.dom,
-   by {apply (pfun.dom_iff_graph c'.val t₁).mpr, exact ⟨q₂, H₂⟩},
-   exact (aux_c''_dom t₁ this).left},
-  {cases H₁; cases H₁; cases H₂; cases H₂, cc},
-  {repeat{cases H₂}, suffices : t₂ ≠ t₂, by contradiction, have : t₂ ∈ c'.val.dom,
-   by {apply (pfun.dom_iff_graph c'.val t₂).mpr, exact ⟨q₁, H₁⟩},
-   exact (aux_c''_dom t₂ this).right},
-  {cases H₂},
-  {repeat{cases H₁}, cases H₂, refl},
-  {cases H₂},
-  {repeat{cases H₁}, suffices : t₂ ≠ t₂, by contradiction, have : t₂ ∈ c'.val.dom,
-   by {apply (pfun.dom_iff_graph c'.val t₂).mpr, refine ⟨_,_⟩, exact q₂, exact H₂},
-   exact (aux_c''_dom t₂ this).right}, {repeat{cases H₂}, cases H₁, refl},
-  {cases H₁}, {cases H₁}, {cc}, {cases H₂}, {cases H₁}, {cases H₁},
-end
-
-/-- the graph of the extension of c by (b₁,m) and (b₂,m) contains the graphs of p₁ and p₂ -/
-lemma one_point_restriction_refinement_extension_graph_extends {p₁ p₂ : cohen_poset} {t₁ t₂ : (set $ set ℕ) × ℕ} (h_t₁ : t₁ ∈ p₁.val.dom) (h_t₂ : t₂ ∈ p₂.val.dom) (q : Prop) (h_val₁ : pfun.fn p₁.val t₁ h_t₁ = q) (h_val₂ : pfun.fn p₂.val t₂ h_t₂ = q) (c : cohen_poset) (h_c_left : c ≤ (one_point_restriction p₁ t₁ h_t₁)) (h_c_right : c ≤ (one_point_restriction p₂ t₂ h_t₂)) : p₁.val.graph ⊆ (one_point_restriction_refinement_extension_graph h_t₁ h_t₂ q h_val₁ h_val₂ c) ∧ p₂.val.graph ⊆ (one_point_restriction_refinement_extension_graph h_t₁ h_t₂ q h_val₁ h_val₂ c) :=
-begin
-  split; intros x Hx; rcases x with ⟨x, q'⟩;
-  dsimp[one_point_restriction_refinement_extension_graph],
-  suffices : ((x, q') ∈ pfun.graph ((aux_c'' h_t₁ h_t₂ q h_val₁ h_val₂ c).val)) ∨ ((x, q') ∈ {(t₁, q)} ∨
-    (x, q') ∈ {(t₂, q)}), by rwa[or_assoc],
-  let H, swap, change _ ∨ H, haveI : decidable H := by apply classical.prop_decidable _,
-  by_cases H,
-    {apply or.elim h, exact λ A, or.inr $ or.inl $ A,
-                      exact λ A, or.inr $ or.inr $ A},
-    {-- dsimp[H] at h, rw[not_or_distrib] at h, apply or.inl,
-    repeat{sorry}
-  
-    -- apply (aux_c''_graph_of (x,q')).mp,
-     -- refine ⟨_, _⟩,
-
--- dsimp[H] at h, rw[not_or_distrib] at h,
---      have Hx' : (x,q') ∈ (c.val).graph,
---        by {apply h_c_left, apply (one_point_restriction_graph (x,q')).mpr,
---        refine ⟨(by assumption), _⟩, change x ≠ t₁, cases h, intro hx, apply h_left, rw[hx], simp,
---               apply (pfun.graph_functional p₁.val), exact Hx,
---               rw[hx], apply (pfun.lift_graph' _).mpr, exact h_val₁},
---      apply or.inl, have : x ∈ p₁.val.dom, by apply (pfun.dom_iff_graph _ x).mpr; exact ⟨q', Hx⟩,
---      have : x ∈ ((aux_c'' h_t₁ h_t₂ q h_val₁ h_val₂ c).val).dom,
---        by {apply aux_c''_dom_of, {split, {change x ≠ t₁, cases h, intro hx,
---           apply h_left, rw[hx], simp, apply (pfun.graph_functional p₁.val), exact Hx,
---           rw[hx], apply (pfun.lift_graph' _).mpr, exact h_val₁}, {change x ≠ t₂, cases h, intro hx, apply h_right, rw[hx], simp, apply (pfun.graph_functional p₂.val), repeat{sorry} -- exact Hx, rw[hx], apply (pfun.lift_graph' _).mpr, exact h_val₂
---               }}, {apply (pfun.dom_iff_graph _ x).mpr, exact ⟨q', Hx'⟩}},
-
-    },
-  -- by_cases H, repeat{sorry}
-  -- have : ((x, q') ∈ {(t₁, q)} ∨ (x, q') ∈ {(t₂, q)}) → (x,q') ∉ pfun.graph ((aux_c'' h_t₁ h_t₂ q h_val₁ h_val₂ c).val),
-  -- by {intros H₁ H₂, have : x ∈ (aux_c'' h_t₁ h_t₂ q h_val₁ h_val₂ c).val.dom,
-  --    by {apply (pfun.dom_iff_graph _ x).mpr, exact ⟨q', H₂⟩}, have := aux_c''_dom x this,
-  --    cases H₁, have : (x,q') = (t₁, q), from set.eq_of_mem_singleton (by assumption), finish,
-  --    have : (x,q') = (t₂, q), from set.eq_of_mem_singleton (by assumption), finish},
-  repeat{sorry}
-  
-end
-
-/-- the extension of c by (b₁, m) and (b₂,m) has finite domain -/
-lemma one_point_restriction_refinement_extension_finite {p₁ p₂ : cohen_poset} {t₁ t₂ : (set $ set ℕ) × ℕ} (h_t₁ : t₁ ∈ p₁.val.dom) (h_t₂ : t₂ ∈ p₂.val.dom) (q : Prop) (h_val₁ : pfun.fn p₁.val t₁ h_t₁ = q) (h_val₂ : pfun.fn p₂.val t₂ h_t₂ = q) (c : cohen_poset) (h_c_left : c ≤ (one_point_restriction p₁ t₁ h_t₁)) (h_c_right : c ≤ (one_point_restriction p₂ t₂ h_t₂)) : set.finite (pfun.of_graph (one_point_restriction_refinement_extension_graph h_t₁ h_t₂ q h_val₁ h_val₂ c) (by {apply one_point_restriction_refinement_extension_graph_functional, repeat{assumption}})).dom :=
-begin
-  unfold one_point_restriction_refinement_extension_graph,
-  rw[pfun.dom_of_graph_union], swap,
-  apply pfun.functional_subset (one_point_restriction_refinement_extension_graph h_t₁ h_t₂ q h_val₁ h_val₂ c),
-    by {unfold one_point_restriction_refinement_extension_graph, finish},
-  apply one_point_restriction_refinement_extension_graph_functional, repeat{assumption},
-  rw[pfun.dom_of_graph_union, pfun.of_graph_graph], simp only [set.union_singleton], repeat{apply set.finite_insert}, apply aux_c''_dom_finite
-end
-
-noncomputable def one_point_restriction_refinement_extension {p₁ p₂ : cohen_poset} {t₁ t₂ : (set $ set ℕ) × ℕ} (h_t₁ : t₁ ∈ p₁.val.dom) (h_t₂ : t₂ ∈ p₂.val.dom) (q : Prop) (h_val₁ : pfun.fn p₁.val t₁ h_t₁ = q) (h_val₂ : pfun.fn p₂.val t₂ h_t₂ = q) (c : cohen_poset) (h_c_left : c ≤ (one_point_restriction p₁ t₁ h_t₁)) (h_c_right : c ≤ (one_point_restriction p₂ t₂ h_t₂)) : cohen_poset :=
-  ⟨pfun.of_graph (one_point_restriction_refinement_extension_graph h_t₁ h_t₂ q h_val₁ h_val₂ c) (by {apply one_point_restriction_refinement_extension_graph_functional, repeat{assumption}}),
-   (by {apply one_point_restriction_refinement_extension_finite, repeat{assumption}})⟩
-
-lemma one_point_restriction_refinement_extension_spec (p₁ p₂ : cohen_poset) {t₁ t₂ : (set $ set ℕ) × ℕ} {h_t₁ : t₁ ∈ p₁.val.dom} {h_t₂ : t₂ ∈ p₂.val.dom} {q : Prop} {h_val₁ : pfun.fn p₁.val t₁ h_t₁ = q} {h_val₂ : pfun.fn p₂.val t₂ h_t₂ = q} {c : cohen_poset} (h_c_left : c ≤ (one_point_restriction p₁ t₁ h_t₁)) (h_c_right : c ≤ (one_point_restriction p₂ t₂ h_t₂)) : ∃ c' : cohen_poset, c' ≤ p₁ ∧ c' ≤ p₂ :=
-begin
-  refine ⟨by {fapply one_point_restriction_refinement_extension h_t₁ h_t₂ q h_val₁ h_val₂ c,
-             repeat{assumption}}, _⟩,
-  have := one_point_restriction_refinement_extension_graph_extends h_t₁ h_t₂ q h_val₁ h_val₂ c h_c_left h_c_right,
-  convert this; convert rfl; simp[one_point_restriction_refinement_extension, one_point_restriction_refinement_extension_graph, pfun.graph_of_graph]
-end
-
-lemma wit_incompatible {p₁ p₂ : cohen_poset} (h_incompat : incompatible p₁ p₂) : ∃ w ∈ p₁.val.dom ∩ p₂.val.dom, pfun.fn (p₁.val) w (by exact H.left) ≠ pfun.fn (p₂.val) w H.right :=
-begin
-  sorry
-  -- let p, swap, change p, haveI : decidable p := by apply classical.prop_decidable _,
-  -- by_contra, dsimp[p] at a, clear _inst p,
-  -- simp at a, sorry
-end
-
-lemma wit_incompatible' {p₁ p₂ : cohen_poset} (h_incompat : incompatible p₁ p₂) : ∃ w q₁ q₂, (w,q₁) ∈ p₁.val.graph ∧ (w,q₂) ∈ p₂.val.graph ∧ q₁ ≠ q₂ := sorry
-
-end one_point_restriction
-
-lemma congr_neq {α β : Type*} {f : α → β} {x' y' : α} {x y : β} {h_x : f x' = x} {h_y : f y' = y} {h_neq : x ≠ y} : x' ≠ y' := λ _, by {cc}
-
-lemma coe_subtype_injective {α : Type*} {s : set α} {x y : s} : (↑x = (↑y : α)) → x = y :=
-  λ h, by {cases x, cases y, dsimp at h, subst h}
-
--- /- The Cohen poset has the countable chain condition -/
--- lemma cohen_poset_ccc : countable_chain_condition cohen_poset :=
+-- lemma aux_c''_dom_of {p₁ p₂ : (@cohen_poset η)} {t₁ t₂ : (set $ set ℕ) × ℕ} {h_t₁ : t₁ ∈ p₁.val.dom} {h_t₂ : t₂ ∈ p₂.val.dom} {q : Prop} {h_val₁ : pfun.fn p₁.val t₁ h_t₁ = q} {h_val₂ : pfun.fn p₂.val t₂ h_t₂ = q} {c : (@cohen_poset η)} : ∀ (x), x ≠ t₁ ∧ x ≠ t₂ → x ∈ c.val.dom → x ∈ (aux_c'' h_t₁ h_t₂ q h_val₁ h_val₂ c).val.dom :=
 -- begin
---   intros a Ha, apply countable_of_countable_fibers' a size_of_domain,
---   intro n, induction n with n ih generalizing a,
---     {apply countable_subsingleton, apply size_of_domain_0_inter_subsingleton},
---     {let A_n, swap, change set.countable A_n,
---       have : A_n ⊆ ⋃ m, is_defined_at m, by {dsimp[A_n], apply inter_subset_right',
---              apply is_defined_at_covers, apply nat.zero_lt_succ},
---      rw[@cover_Union_eq _ _ A_n is_defined_at this], apply set.countable_Union,
---      intro m, let A_n_m, swap, change set.countable A_n_m,
---        have choice_aux : ∀ p : A_n_m, ∃ b : (set $ set ℕ), (b,m) ∈ (pfun.dom p.val.val),
---          by {intros p, cases p, cases p_property, cases p_val, assumption},
---        have := classical.axiom_of_choice choice_aux, cases this with wit wit_spec,
---        let eval : A_n_m → Prop :=
---              λ (p : ↥A_n_m), pfun.fn ((p.val).val) (wit p, m) (by apply wit_spec),
---        apply countable_of_countable_fibers'' _ eval, intro q,
---        let A_n_m_q, swap, change set.countable A_n_m_q,
+--   intros x Hx H'x, rcases Hx with ⟨Hx_r, Hx_l⟩, dsimp[aux_c''],
+--   repeat{rw[one_point_restriction_domain']}, finish
+-- end
+
+-- lemma aux_c''_graph_of {p₁ p₂ : (@cohen_poset η)} {t₁ t₂ : (set $ set ℕ) × ℕ} {h_t₁ : t₁ ∈ p₁.val.dom} {h_t₂ : t₂ ∈ p₂.val.dom} {q : Prop} {h_val₁ : pfun.fn p₁.val t₁ h_t₁ = q} {h_val₂ : pfun.fn p₂.val t₂ h_t₂ = q} {c : (@cohen_poset η)} : ∀ x, (x ∈ c.val.graph ∧ (prod.fst x ≠ t₁ ) ∧ (prod.fst x ≠ t₂)) ↔ x ∈ (aux_c'' h_t₁ h_t₂ q h_val₁ h_val₂ c).val.graph := sorry
+
+-- lemma aux_c''_dom_finite {p₁ p₂ : (@cohen_poset η)} {t₁ t₂ : (set $ set ℕ) × ℕ} {h_t₁ : t₁ ∈ p₁.val.dom} {h_t₂ : t₂ ∈ p₂.val.dom} {q : Prop} {h_val₁ : pfun.fn p₁.val t₁ h_t₁ = q} {h_val₂ : pfun.fn p₂.val t₂ h_t₂ = q} {c : (@cohen_poset η)} : set.finite (aux_c'' h_t₁ h_t₂ q h_val₁ h_val₂ c).val.dom :=
+-- begin
+--   dsimp[aux_c''], repeat{rw[one_point_restriction_domain']}, repeat{apply finite_of_inter_not_x},
+--   exact c.property
+-- end
+-- -- λ x Hx, ⟨by {apply ((in_one_point_restriction'_of_in_dom_and_not_x).mp _).right, exact c,
+-- --             apply one_point_restriction_domain'_subset, swap, exact t₂, exact Hx},
+-- --          by {apply ((in_one_point_restriction'_of_in_dom_and_not_x).mp _).right, exact (one_point_restriction' c t₁), exact Hx}⟩
+
+-- /- Let p₁ and p₂ be two partial functions such that there is a point (b₁,m) for p₁ and a point (b₂, m) for p₂ where p₁ and p₂ have the same value.
+--     Suppose that the one-point restrictions of p₁ and p₂ with respect to (b₁,m) and (b₂,m) have a common refinement c.
+--     Then c (after making sure (b₁, m) and (b₂,m) are not in its domain) extended by (b₁,m) and (b₂,m) is a common refinement for p₁ and p₂. -/
+
+-- /-- the graph of the extension of c by (b₁,m) and (b₂,m) -/
+-- def one_point_restriction_refinement_extension_graph {p₁ p₂ : (@cohen_poset η)} {t₁ t₂ : (set $ set ℕ) × ℕ} (h_t₁ : t₁ ∈ p₁.val.dom) (h_t₂ : t₂ ∈ p₂.val.dom) (q : Prop) (h_val₁ : pfun.fn p₁.val t₁ h_t₁ = q) (h_val₂ : pfun.fn p₂.val t₂ h_t₂ = q) (c : (@cohen_poset η)) :=
+--   ((aux_c'' h_t₁ h_t₂ q h_val₁ h_val₂ c).val.graph ∪ {(t₁,q)} ∪ {(t₂,q)})
+
+-- lemma one_point_restriction_refinement_extension_graph_functional {p₁ p₂ : (@cohen_poset η)} {t₁ t₂ : (set $ set ℕ) × ℕ} (h_t₁ : t₁ ∈ p₁.val.dom) (h_t₂ : t₂ ∈ p₂.val.dom) (q : Prop) (h_val₁ : pfun.fn p₁.val t₁ h_t₁ = q) (h_val₂ : pfun.fn p₂.val t₂ h_t₂ = q) (c : (@cohen_poset η)) (h_c_left : c ≤ (one_point_restriction p₁ t₁ h_t₁)) (h_c_right : c ≤ (one_point_restriction p₂ t₂ h_t₂)) :
+--   pfun.functional $ one_point_restriction_refinement_extension_graph h_t₁ h_t₂ q h_val₁ h_val₂ c :=
+-- begin
+--   intros x q₁ q₂ H₁ H₂, let c' := (aux_c'' h_t₁ h_t₂ q h_val₁ h_val₂ c), cases H₁; cases H₂; cases H₁; cases H₂,
+--   apply pfun.graph_functional (aux_c'' h_t₁ h_t₂ q h_val₁ h_val₂ c).val, exact H₁, exact H₂,
+--   {have : x ∈ c'.val.dom,
+--     by {apply (pfun.dom_iff_graph c'.val x).mpr, exact ⟨q₁, H₁⟩}, have := (aux_c''_dom x this).left, suffices : x = t₁, by contradiction, repeat{cases H₂}, refl},
+--   {repeat{cases H₁}, suffices : t₁ ≠ t₁, by contradiction, have : t₁ ∈ c'.val.dom,
+--    by {apply (pfun.dom_iff_graph c'.val t₁).mpr, exact ⟨q₂, H₂⟩},
+--    exact (aux_c''_dom t₁ this).left},
+--   {cases H₁; cases H₁; cases H₂; cases H₂, cc},
+--   {repeat{cases H₂}, suffices : t₂ ≠ t₂, by contradiction, have : t₂ ∈ c'.val.dom,
+--    by {apply (pfun.dom_iff_graph c'.val t₂).mpr, exact ⟨q₁, H₁⟩},
+--    exact (aux_c''_dom t₂ this).right},
+--   {cases H₂},
+--   {repeat{cases H₁}, cases H₂, refl},
+--   {cases H₂},
+--   {repeat{cases H₁}, suffices : t₂ ≠ t₂, by contradiction, have : t₂ ∈ c'.val.dom,
+--    by {apply (pfun.dom_iff_graph c'.val t₂).mpr, refine ⟨_,_⟩, exact q₂, exact H₂},
+--    exact (aux_c''_dom t₂ this).right}, {repeat{cases H₂}, cases H₁, refl},
+--   {cases H₁}, {cases H₁}, {cc}, {cases H₂}, {cases H₁}, {cases H₁},
+-- end
+
+-- /-- the graph of the extension of c by (b₁,m) and (b₂,m) contains the graphs of p₁ and p₂ -/
+-- lemma one_point_restriction_refinement_extension_graph_extends {p₁ p₂ : (@cohen_poset η)} {t₁ t₂ : (set $ set ℕ) × ℕ} (h_t₁ : t₁ ∈ p₁.val.dom) (h_t₂ : t₂ ∈ p₂.val.dom) (q : Prop) (h_val₁ : pfun.fn p₁.val t₁ h_t₁ = q) (h_val₂ : pfun.fn p₂.val t₂ h_t₂ = q) (c : (@cohen_poset η)) (h_c_left : c ≤ (one_point_restriction p₁ t₁ h_t₁)) (h_c_right : c ≤ (one_point_restriction p₂ t₂ h_t₂)) : p₁.val.graph ⊆ (one_point_restriction_refinement_extension_graph h_t₁ h_t₂ q h_val₁ h_val₂ c) ∧ p₂.val.graph ⊆ (one_point_restriction_refinement_extension_graph h_t₁ h_t₂ q h_val₁ h_val₂ c) :=
+-- begin
+--   split; intros x Hx; rcases x with ⟨x, q'⟩;
+--   dsimp[one_point_restriction_refinement_extension_graph],
+--   suffices : ((x, q') ∈ pfun.graph ((aux_c'' h_t₁ h_t₂ q h_val₁ h_val₂ c).val)) ∨ ((x, q') ∈ {(t₁, q)} ∨
+--     (x, q') ∈ {(t₂, q)}), by rwa[or_assoc],
+--   let H, swap, change _ ∨ H, haveI : decidable H := by apply classical.prop_decidable _,
+--   by_cases H,
+--     {apply or.elim h, exact λ A, or.inr $ or.inl $ A,
+--                       exact λ A, or.inr $ or.inr $ A},
+--     {-- dsimp[H] at h, rw[not_or_distrib] at h, apply or.inl,
+--     repeat{sorry}
+  
+--     -- apply (aux_c''_graph_of (x,q')).mp,
+--      -- refine ⟨_, _⟩,
+
+-- -- dsimp[H] at h, rw[not_or_distrib] at h,
+-- --      have Hx' : (x,q') ∈ (c.val).graph,
+-- --        by {apply h_c_left, apply (one_point_restriction_graph (x,q')).mpr,
+-- --        refine ⟨(by assumption), _⟩, change x ≠ t₁, cases h, intro hx, apply h_left, rw[hx], simp,
+-- --               apply (pfun.graph_functional p₁.val), exact Hx,
+-- --               rw[hx], apply (pfun.lift_graph' _).mpr, exact h_val₁},
+-- --      apply or.inl, have : x ∈ p₁.val.dom, by apply (pfun.dom_iff_graph _ x).mpr; exact ⟨q', Hx⟩,
+-- --      have : x ∈ ((aux_c'' h_t₁ h_t₂ q h_val₁ h_val₂ c).val).dom,
+-- --        by {apply aux_c''_dom_of, {split, {change x ≠ t₁, cases h, intro hx,
+-- --           apply h_left, rw[hx], simp, apply (pfun.graph_functional p₁.val), exact Hx,
+-- --           rw[hx], apply (pfun.lift_graph' _).mpr, exact h_val₁}, {change x ≠ t₂, cases h, intro hx, apply h_right, rw[hx], simp, apply (pfun.graph_functional p₂.val), repeat{sorry} -- exact Hx, rw[hx], apply (pfun.lift_graph' _).mpr, exact h_val₂
+-- --               }}, {apply (pfun.dom_iff_graph _ x).mpr, exact ⟨q', Hx'⟩}},
+
+--     },
+--   -- by_cases H, repeat{sorry}
+--   -- have : ((x, q') ∈ {(t₁, q)} ∨ (x, q') ∈ {(t₂, q)}) → (x,q') ∉ pfun.graph ((aux_c'' h_t₁ h_t₂ q h_val₁ h_val₂ c).val),
+--   -- by {intros H₁ H₂, have : x ∈ (aux_c'' h_t₁ h_t₂ q h_val₁ h_val₂ c).val.dom,
+--   --    by {apply (pfun.dom_iff_graph _ x).mpr, exact ⟨q', H₂⟩}, have := aux_c''_dom x this,
+--   --    cases H₁, have : (x,q') = (t₁, q), from set.eq_of_mem_singleton (by assumption), finish,
+--   --    have : (x,q') = (t₂, q), from set.eq_of_mem_singleton (by assumption), finish},
+--   repeat{sorry}
+  
+-- end
+
+-- /-- the extension of c by (b₁, m) and (b₂,m) has finite domain -/
+-- lemma one_point_restriction_refinement_extension_finite {p₁ p₂ : (@cohen_poset η)} {t₁ t₂ : (set $ set ℕ) × ℕ} (h_t₁ : t₁ ∈ p₁.val.dom) (h_t₂ : t₂ ∈ p₂.val.dom) (q : Prop) (h_val₁ : pfun.fn p₁.val t₁ h_t₁ = q) (h_val₂ : pfun.fn p₂.val t₂ h_t₂ = q) (c : (@cohen_poset η)) (h_c_left : c ≤ (one_point_restriction p₁ t₁ h_t₁)) (h_c_right : c ≤ (one_point_restriction p₂ t₂ h_t₂)) : set.finite (pfun.of_graph (one_point_restriction_refinement_extension_graph h_t₁ h_t₂ q h_val₁ h_val₂ c) (by {apply one_point_restriction_refinement_extension_graph_functional, repeat{assumption}})).dom :=
+-- begin
+--   unfold one_point_restriction_refinement_extension_graph,
+--   rw[pfun.dom_of_graph_union], swap,
+--   apply pfun.functional_subset (one_point_restriction_refinement_extension_graph h_t₁ h_t₂ q h_val₁ h_val₂ c),
+--     by {unfold one_point_restriction_refinement_extension_graph, finish},
+--   apply one_point_restriction_refinement_extension_graph_functional, repeat{assumption},
+--   rw[pfun.dom_of_graph_union, pfun.of_graph_graph], simp only [set.union_singleton], repeat{apply set.finite_insert}, apply aux_c''_dom_finite
+-- end
+
+-- noncomputable def one_point_restriction_refinement_extension {p₁ p₂ : (@cohen_poset η)} {t₁ t₂ : (set $ set ℕ) × ℕ} (h_t₁ : t₁ ∈ p₁.val.dom) (h_t₂ : t₂ ∈ p₂.val.dom) (q : Prop) (h_val₁ : pfun.fn p₁.val t₁ h_t₁ = q) (h_val₂ : pfun.fn p₂.val t₂ h_t₂ = q) (c : (@cohen_poset η)) (h_c_left : c ≤ (one_point_restriction p₁ t₁ h_t₁)) (h_c_right : c ≤ (one_point_restriction p₂ t₂ h_t₂)) : (@cohen_poset η) :=
+--   ⟨pfun.of_graph (one_point_restriction_refinement_extension_graph h_t₁ h_t₂ q h_val₁ h_val₂ c) (by {apply one_point_restriction_refinement_extension_graph_functional, repeat{assumption}}),
+--    (by {apply one_point_restriction_refinement_extension_finite, repeat{assumption}})⟩
+
+-- lemma one_point_restriction_refinement_extension_spec (p₁ p₂ : (@cohen_poset η)) {t₁ t₂ : (set $ set ℕ) × ℕ} {h_t₁ : t₁ ∈ p₁.val.dom} {h_t₂ : t₂ ∈ p₂.val.dom} {q : Prop} {h_val₁ : pfun.fn p₁.val t₁ h_t₁ = q} {h_val₂ : pfun.fn p₂.val t₂ h_t₂ = q} {c : (@cohen_poset η)} (h_c_left : c ≤ (one_point_restriction p₁ t₁ h_t₁)) (h_c_right : c ≤ (one_point_restriction p₂ t₂ h_t₂)) : ∃ c' : (@cohen_poset η), c' ≤ p₁ ∧ c' ≤ p₂ :=
+-- begin
+--   refine ⟨by {fapply one_point_restriction_refinement_extension h_t₁ h_t₂ q h_val₁ h_val₂ c,
+--              repeat{assumption}}, _⟩,
+--   have := one_point_restriction_refinement_extension_graph_extends h_t₁ h_t₂ q h_val₁ h_val₂ c h_c_left h_c_right,
+--   convert this; convert rfl; simp[one_point_restriction_refinement_extension, one_point_restriction_refinement_extension_graph, pfun.graph_of_graph]
+-- end
+
+-- lemma wit_incompatible {p₁ p₂ : (@cohen_poset η)} (h_incompat : incompatible p₁ p₂) : ∃ w ∈ p₁.val.dom ∩ p₂.val.dom, pfun.fn (p₁.val) w (by exact H.left) ≠ pfun.fn (p₂.val) w H.right :=
+-- begin
+--   sorry
+--   -- let p, swap, change p, haveI : decidable p := by apply classical.prop_decidable _,
+--   -- by_contra, dsimp[p] at a, clear _inst p,
+--   -- simp at a, sorry
+-- end
+
+-- lemma wit_incompatible' {p₁ p₂ : (@cohen_poset η)} (h_incompat : incompatible p₁ p₂) : ∃ w q₁ q₂, (w,q₁) ∈ p₁.val.graph ∧ (w,q₂) ∈ p₂.val.graph ∧ q₁ ≠ q₂ := sorry
+
+-- end one_point_restriction
+
+-- lemma congr_neq {α β : Type*} {f : α → β} {x' y' : α} {x y : β} {h_x : f x' = x} {h_y : f y' = y} {h_neq : x ≠ y} : x' ≠ y' := λ _, by {cc}
+
+-- lemma coe_subtype_injective {α : Type*} {s : set α} {x y : s} : (↑x = (↑y : α)) → x = y :=
+--   λ h, by {cases x, cases y, dsimp at h, subst h}
+
+-- -- /- The Cohen poset has the countable chain condition -/
+-- -- lemma (@cohen_poset η)_ccc : countable_chain_condition (@cohen_poset η) :=
+-- -- begin
+-- --   intros a Ha, apply countable_of_countable_fibers' a size_of_domain,
+-- --   intro n, induction n with n ih generalizing a,
+-- --     {apply countable_subsingleton, apply size_of_domain_0_inter_subsingleton},
+-- --     {let A_n, swap, change set.countable A_n,
+-- --       have : A_n ⊆ ⋃ m, is_defined_at m, by {dsimp[A_n], apply inter_subset_right',
+-- --              apply is_defined_at_covers, apply nat.zero_lt_succ},
+-- --      rw[@cover_Union_eq _ _ A_n is_defined_at this], apply set.countable_Union,
+-- --      intro m, let A_n_m, swap, change set.countable A_n_m,
+-- --        have choice_aux : ∀ p : A_n_m, ∃ b : (set $ set ℕ), (b,m) ∈ (pfun.dom p.val.val),
+-- --          by {intros p, cases p, cases p_property, cases p_val, assumption},
+-- --        have := classical.axiom_of_choice choice_aux, cases this with wit wit_spec,
+-- --        let eval : A_n_m → Prop :=
+-- --              λ (p : ↥A_n_m), pfun.fn ((p.val).val) (wit p, m) (by apply wit_spec),
+-- --        apply countable_of_countable_fibers'' _ eval, intro q,
+-- --        let A_n_m_q, swap, change set.countable A_n_m_q,
      
---          let red : A_n_m → cohen_poset :=
---            λ X, one_point_restriction X.val (wit X, m) (by apply wit_spec),
+-- --          let red : A_n_m → (@cohen_poset η) :=
+-- --            λ X, one_point_restriction X.val (wit X, m) (by apply wit_spec),
 
---          have h_anti : antichain (red '' A_n_m_q) :=
---            by {intros x H_x y H_y H_neq H_compat, rcases H_compat with ⟨c, ⟨H_cx,H_cy⟩⟩,
---                rcases H_x with ⟨x', H_x'⟩, rcases H_y with ⟨y', H_y'⟩,
---                have h_neq : x' ≠ y',
---                  by {apply congr_neq, exact H_x'.right, exact H_y'.right, exact H_neq},
---                have : ↑x' ≠ ↑y', by {intro, apply h_neq, exact coe_subtype_injective a_1},
---                have h_incompat := Ha x' (x'.property.left.right) y' (y'.property.left.right) this,
---                have := wit_incompatible' h_incompat, rcases this with ⟨w,q₁,q₂, ⟨H₁,⟨H₂,H₃⟩⟩⟩,
---                have w_not_t₁ : w ≠ (wit (x'), m),
---                  by {intro H_eq, have := pfun.congr_arg (subtype.val (↑x'))
---                                          (pfun.in_dom_of_in_graph (by assumption))
---                                          (pfun.in_dom_of_in_graph (sorry)) H_eq, repeat{sorry}
---                      },
---                have w_not_t₂ : w.fst ≠ wit (y'), by sorry,
---                have w_in_red_1 : (w,q₁) ∈ (x).val.graph, by sorry,
---                have w_in_red_2 : (w,q₂) ∈ (y).val.graph, by sorry,
---                have w_in_c_1 : (w,q₁) ∈ c.val.graph, from H_cx w_in_red_1,
---                have w_in_c_2 : (w,q₂) ∈ c.val.graph, from H_cy w_in_red_2,
---                suffices : q₁ = q₂, by contradiction,
---                apply pfun.graph_functional c.val, exacts [w_in_c_1, w_in_c_2]
---                },
+-- --          have h_anti : antichain (red '' A_n_m_q) :=
+-- --            by {intros x H_x y H_y H_neq H_compat, rcases H_compat with ⟨c, ⟨H_cx,H_cy⟩⟩,
+-- --                rcases H_x with ⟨x', H_x'⟩, rcases H_y with ⟨y', H_y'⟩,
+-- --                have h_neq : x' ≠ y',
+-- --                  by {apply congr_neq, exact H_x'.right, exact H_y'.right, exact H_neq},
+-- --                have : ↑x' ≠ ↑y', by {intro, apply h_neq, exact coe_subtype_injective a_1},
+-- --                have h_incompat := Ha x' (x'.property.left.right) y' (y'.property.left.right) this,
+-- --                have := wit_incompatible' h_incompat, rcases this with ⟨w,q₁,q₂, ⟨H₁,⟨H₂,H₃⟩⟩⟩,
+-- --                have w_not_t₁ : w ≠ (wit (x'), m),
+-- --                  by {intro H_eq, have := pfun.congr_arg (subtype.val (↑x'))
+-- --                                          (pfun.in_dom_of_in_graph (by assumption))
+-- --                                          (pfun.in_dom_of_in_graph (sorry)) H_eq, repeat{sorry}
+-- --                      },
+-- --                have w_not_t₂ : w.fst ≠ wit (y'), by sorry,
+-- --                have w_in_red_1 : (w,q₁) ∈ (x).val.graph, by sorry,
+-- --                have w_in_red_2 : (w,q₂) ∈ (y).val.graph, by sorry,
+-- --                have w_in_c_1 : (w,q₁) ∈ c.val.graph, from H_cx w_in_red_1,
+-- --                have w_in_c_2 : (w,q₂) ∈ c.val.graph, from H_cy w_in_red_2,
+-- --                suffices : q₁ = q₂, by contradiction,
+-- --                apply pfun.graph_functional c.val, exacts [w_in_c_1, w_in_c_2]
+-- --                },
 
---          have ih_rewrite : size_of_domain ⁻¹' {n} ∩ red '' A_n_m_q = red '' A_n_m_q,
---            by {apply set.inter_eq_self_of_subset_right, intros x H_x,
---               simp only [set.mem_singleton_iff, set.mem_preimage_eq],
---               dsimp[red] at H_x, cases H_x, rw[<-H_x_h.right],
---               apply one_point_restriction_decrease_size,
---               apply size_of_domain_fiber H_x_w.property.left.left},
+-- --          have ih_rewrite : size_of_domain ⁻¹' {n} ∩ red '' A_n_m_q = red '' A_n_m_q,
+-- --            by {apply set.inter_eq_self_of_subset_right, intros x H_x,
+-- --               simp only [set.mem_singleton_iff, set.mem_preimage_eq],
+-- --               dsimp[red] at H_x, cases H_x, rw[<-H_x_h.right],
+-- --               apply one_point_restriction_decrease_size,
+-- --               apply size_of_domain_fiber H_x_w.property.left.left},
 
---          have h_inj : set.inj_on red A_n_m_q,
---            by {intros x' y' H_x' H_y',
---               haveI : decidable_eq ↥A_n_m := λ _ _, classical.prop_decidable _,
---               by_cases x' = y', exact λ _, ‹x' = y'›, rename h h_neq,
---               intro H, exfalso, 
---                refine Ha x' (x'.property.left.right) y' (y'.property.left.right)
---                            (by {intro, apply h_neq, exact coe_subtype_injective a_1}) _,
---               apply one_point_restriction_refinement_extension_spec (↑x') (↑y'),
---               have : red x' ≤ red x', by {apply le_of_eq rfl},
---               convert this, convert (le_of_eq H), exact q,
---                cases H_x', convert H_x', cases H_x',
---                cases H_y', convert H_y', cases H_y'},
+-- --          have h_inj : set.inj_on red A_n_m_q,
+-- --            by {intros x' y' H_x' H_y',
+-- --               haveI : decidable_eq ↥A_n_m := λ _ _, classical.prop_decidable _,
+-- --               by_cases x' = y', exact λ _, ‹x' = y'›, rename h h_neq,
+-- --               intro H, exfalso, 
+-- --                refine Ha x' (x'.property.left.right) y' (y'.property.left.right)
+-- --                            (by {intro, apply h_neq, exact coe_subtype_injective a_1}) _,
+-- --               apply one_point_restriction_refinement_extension_spec (↑x') (↑y'),
+-- --               have : red x' ≤ red x', by {apply le_of_eq rfl},
+-- --               convert this, convert (le_of_eq H), exact q,
+-- --                cases H_x', convert H_x', cases H_x',
+-- --                cases H_y', convert H_y', cases H_y'},
 
---          have ih' := ih (red '' A_n_m_q) h_anti,
+-- --          have ih' := ih (red '' A_n_m_q) h_anti,
 
---          exact set.countable_of_injective_of_countable_image h_inj (by rwa[<-ih_rewrite])}
+-- --          exact set.countable_of_injective_of_countable_image h_inj (by rwa[<-ih_rewrite])}
 -- end
